\subsection{Differential Forms}
We had earlier seen 1-forms when dealing with covectors. We will now discuss about their generalisations
\begin{definition}[Differential Form]
    A differential $k$-form  $\omega$ on a manifold $\SM$ is an antisymmetric differentiable $\mqty(0\\k)$ tensor field on $\SM$
\end{definition}
Antisymmetric property simply means that if two inputs are exchanged, the outputs become negative of one another, that is,
$$\omega(X_1,\ldots X_i\ldots X_j \ldots X_k)= -\omega(X_1,\ldots X_j\ldots X_i \ldots X_k) \ \ X_i\in\mathfrak{X}(\SM)$$
An immediate consequence is that if $\omega$ has two identical arguments, then the result is zero. \\[0.2cm]
A $0$-form is just a function in $\cty{\SM}$ where anytisymmetry is trivial (since no argument is there to input)\\[0.2cm]
If $t$ is a smooth $\mqty(0\\k)$ tensor field, we define $\SA t$ by:
$$\SA t(X_1,\ldots,X_k) = \frac{1}{k!}\sum\limits_{\sigma \in S_k}\mathrm{sgn}(\sigma)t(X_{\sigma(1)},\ldots,X_{\sigma(k)})$$
Note that if we exchange any $X_i$ and $X_j$, then $\mathrm{sgn}(\sigma)$ changes to $-\mathrm{sgn}(\sigma)$ and we obtain a minus sign. Hence, by construction, $\SA t$ is completely anti-symmetric and hence a $k$-form. The operator $\SA$ is called the \textit{alternating operator}. \\[0.2cm]
\textbf{Properties:}
\begin{itemize}
    \item If $t$ and $s$ are both $\mqty(0\\k)$ tensor fields, then $\SA ( t+s) = \SA t + \SA s$
    \item If $t$ is a $\mqty(0\\k)$ tensor field and $f:\SM\rightarrow \re$, then $\SA (ft) = f\SA t$
    \item If $t$ is antisymmetric itself, then $\SA t= t \implies \SA^2 = \SA$
\end{itemize}
The set of all $k$-forms on $\SM$, $\Lambda^k(\SM)$, is a submodule of $T_k^0\SM$. Note that a tensor product of a $k$-form and a $l-$form is not any form in general (since, of the $k+l$ vectors, first $k$ are antisymmetric among themselves and so are the last $l$ but antisymmetricity is not guaranteed among these two sectors). To compnensate for this, we define some other kind of product instead of leaving the fact alone. 
\begin{definition}
    If $\omega$ is a $k$-form and $\eta$ is a $l$-form on $\SM$, then we define the \textit{wedge} or the \textit{exterior} product by:
    $$\ext{\omega}{\eta} = \SA(\omega \otimes \eta)$$
\end{definition}
So basically, we product a $\mqty(0\\k+l)$ tensor field and then antisymmetrise it using the alternating operator to obtain a $(k+l)$  form.\footnote{An alternate definition of the wedge product uses $\ext{\omega}{\eta} =\frac{(k+l)!}{k!l!} \SA(\omega \otimes \eta)$}\\[0.2cm]
\begin{itemize}
    \item \textcolor{blue}{Commutativity}: Note that if $f\in\cty{\SM}$, it is a $\mqty(0\\0)$ tensor field and then for a $k$-form $\omega$, $$\ext{f}{\omega} = \SA(d\otimes \omega) = \SA(f\omega)=f\SA \omega = f\omega = \ext{\omega}{f}$$
    In this case, this is commutative but is not in general always the case. For example, take two $1$-forms $\alpha,\beta$. Then, note that by definition:
    \begin{align*}
        \ext{\alpha}{\beta}(X_1,X_2) &= \SA(\alpha\otimes \beta)(X_1,X_2)\\
        &=\frac{1}{2!}\qty((\alpha\otimes \beta)(X_1,X_2)-(\alpha\otimes \beta)(X_2,X_1))\\
        &=\frac{1}{2}\qty((\alpha\otimes \beta)(X_1,X_2)-(\beta\otimes \alpha)(X_1,X_2))\\
        &=\frac{1}{2}(\alpha\otimes \beta - \beta\otimes \alpha) (X_1,X_2)
    \end{align*}
    This implies $ \ext{\alpha}{\beta} = \frac{1}{2}(\alpha\otimes \beta - \beta\otimes \alpha) = \ext{\beta}{\alpha}$. The third line comes because:
    $$\alpha\otimes \beta (X_2,X_1) = \alpha(X_2)\beta(X_1) = \beta(X_1)\alpha(X_2)=(\beta\otimes \alpha)(X_1,X_2)$$
    The general result is:\begin{lemma}
        If $\alpha\in \Lambda^k\SM$ and $\beta\in \Lambda^l\SM$ then,
    $$\ext{\alpha}{\beta} = (-1)^{kl}\ \ext{\beta}{\alpha}$$
    \end{lemma}
    \textit{Proof.} This is going to be a long (and perhaps inelegant) proof!\\[0.2cm]
    Consider a chart $(U,\phi)$ with coordinate $(x^1,\ldots,x^n)$. Then, since the $k$-form is a $\mqty(0\\k)$ tensor field, we can write it as:
    $$\omega  = \omega_{i_1\ldots i_k}dx^{i_1}\otimes\ldots\otimes dx^{i_k}\qquad \omega_{i_1\ldots i_k} \equiv \omega\qty(\pdv{x^{i_1}},\ldots,\pdv{x^{i_k}})$$
    Since $\omega$ is $k$-form, it will be antisymmetric in all its indices, which implies that $\omega = \SA \omega$, which gives:
    \begin{align*}
          \omega &= \SA(\omega_{i_1\ldots i_k}dx^{i_1}\otimes\ldots\otimes dx^{i_k}) \\
          &=\omega_{i_1\ldots i_k} \SA(dx^{i_1}\otimes\ldots\otimes dx^{i_k})\\
          &=\omega_{i_1\ldots i_k} \ext{dx^{i_1}}{\ext{\ldots}{dx^{i_k}} }
    \end{align*}

    Now consider $\eta = \eta_{j_1\ldots j_k}\ext{dx^{j_1}}{\ext{\ldots}{dx^{j_l}}}$. We will analyse the exterior product of $\eta$ and $\omega$. We also note one fact, that the exterior product is anticommutative in each index, so interchanging one index with introduce an overall minus sign. 
    \begin{align*}
        \ext{\omega}{\eta} &= \ext{ (\omega_{i_1\ldots i_k} \ext{dx^{i_1}}{\ext{\ldots}{dx^{i_k}} }) }{(\eta_{j_1\ldots j_l} \ext{dx^{j_1}}{\ext{\ldots}{dx^{j_l}} })}\\
        &=\omega_{i_1\ldots i_k}  \eta_{j_1\ldots j_l}\ext{ (\ext{dx^{i_1}}{\ext{\ldots}{dx^{i_k}} }) }{( \ext{dx^{j_1}}{\ext{\ldots}{dx^{j_l}} })} \\
        &=\omega_{i_1\ldots i_k}  \eta_{j_1\ldots j_l} (-1)^{kl}\ext{( \ext{dx^{j_1}}{\ext{\ldots}{dx^{j_l}} })} { (\ext{dx^{i_1}}{\ext{\ldots}{dx^{i_k}} }) }\\
        &=(-1)^{kl}\ext{\eta}{\omega}
    \end{align*}
    In the second last line, since there are $l$ terms in the second bracket and to find $\ext{\eta}{\omega}$, we had to move these $l$ terms forward by $k$ places, thus, we get an overall factor of $(-1)^{kl}$
    \item \textcolor{blue}{Linearity}: If $a,b\in \re$ and $\omega_1, \omega_2 \in \Lambda^k\SM, \eta \in \Lambda^l\SM, f\in \cty{\SM}$, then
    $$\ext{(a\omega_1 + b\omega_2)}{\eta} = a\ext{\omega_1}{\eta}+b\ext{\omega_2}{\eta}$$ 
    $$\ext{(f\omega_1)}{\eta} = \ext{\omega_1}{(f\eta)}=f(\ext{\omega}{\eta})$$
    \item \textcolor{blue}{Associativity:} If $\alpha,\beta,\gamma$ are three forms, then:
    $$\ext{\alpha}{(\ext{\beta}{\gamma})} = \ext{(\ext{\alpha}{\beta})}{\gamma}= \ext{\alpha}{\ext{\beta}{\gamma}} = \SA(\alpha\otimes\beta\otimes\gamma)$$
\end{itemize}
\textbf{Example:}\\[0.2cm]
Let $\SM = \re^3$ and the chart $(\SM,\mathrm{id})$. Then we can have maximum upto $3$-form. The basis for each is:
\begin{itemize}
    \item $\Lambda^1\SM\rightarrow dx,dy,dz$,  so any $1$-form $\alpha $ is written as $\alpha = pdx+qdy+rdz$
    \item  $\Lambda^2\SM\rightarrow \ext{dx}{dy},\ext{dy}{dz},\ext{dz}{dx}$ \footnote{Note that any other combination of the wedge product can be written in terms of these}, so any $2$-form $\alpha $ is written as $\alpha = p( \ext{dx}{dy})+q(\ext{dy}{dz})+r(\ext{dz}{dx})$
    \item $\Lambda^2\SM\rightarrow \ext{dx}{\ext{dy}{dz}}$, so any $3$-form $\alpha $ is written as $\alpha =p (\ext{dx}{\ext{dy}{dz}})$
\end{itemize}
Let us now calculate the exterior product of two one forms which can be written as:
\begin{align*}
    p &= p_x dx + p_y dy+p_zdz\\
    q &= q_x dx + q_y dy+q_zdz
\end{align*}
Then we will have:
\begin{align*}
    \ext{p}{q} &= \ext{( p_x dx + p_y dy+p_zdz)}{(q_x dx + q_y dy+q_zdz)}\\
    &=\mathcolor{blue}{p_xq_y \ext{dx}{dy} + p_yq_x \ext{dy}{dx}} + \mathcolor{red}{p_xq_z\ext{dx}{dz} + p_zq_x\ext{dz}{dx}}+\mathcolor{OliveGreen}{p_yq_z\ext{dy}{dz} + p_z q_y\ext{dz}{dy}}\\
    &=(p_xq_y - p_yq_x)\ext{dx}{dy} + (p_xq_z-p_zq_x)\ext{dx}{dz}+ (p_yq_z - p_zq_y)\ext{dy}{dz}\\
    &=(p_xq_y - p_yq_x)\ext{dx}{dy} + (p_zq_x-p_xq_z)\ext{dz}{dx} + (p_yq_z - p_zq_y)\ext{dy}{dz}
\end{align*}
The last term is obtained by interchanging the wedge product in the second term of each coloured term. Notice the familiarity of the components with that of the components of the \textit{cross product}\footnote{We arranged the indices to follow a cyclic pattern like $x\rightarrow y \rightarrow z \rightarrow x$} that we all know. So, we see that the wedge product between two one forms generalises the cross product in some sense. \\[0.2cm]
Let $p = p_x dx + p_y dy+p_zdz$ be a $1$-form and $q = q_x(\ext{dy}{dz})+q_y(\ext{dz}{dx})+q_z( \ext{dx}{dy}) $ be a $2$-form.
\begin{align*}
    \ext{p}{q} &= \ext{(p_x dx + p_y dy+p_zdz)}{(q_x(\ext{dy}{dz})+q_y(\ext{dz}{dx})+q_z( \ext{dx}{dy}))}\\
    &= p_xq_x\ext{dx}{\ext{dy}{dz}}+ p_yq_y \ext{dy}{\ext{dz}{dx}}+p_zq_z\ext{dz}{\ext{dx}{dy}}\\
    &=(p_xq_x+p_yq_y+p_zq_z)\ext{dx}{\ext{dy}{dz}}
\end{align*}
The component is exactly the dot product as we know, and hence the exterior product of a one-form and a two-form generalises the dot product. 
\subsubsection{Exterior Derivative}
\begin{definition}[Exterior Derivative]
    If $\omega$ is a $k$-form, then the exterior derivative of $\omega$, denoted by $d\omega$, is a $(k+1)$-form and is given by:
    \begin{align*}
        d\omega (X_1,\ldots, X_{k+1})&:=\frac{1}{k+1}\Bigg[\sum\limits_{i=1}^{k+1} (-1)^{i+1}X_i \omega(X_1,\ldots \hat{X}_i\ldots,X_{k+1})\\&\qquad\qquad+\sum\limits_{i<j}(-1)^{i+j}\omega(\comtr{X_i}{X_j},X_1,\ldots \hat{X}_i\ldots \hat{X}_j \ldots X_{k+1})\Bigg]
    \end{align*}
\end{definition}
The hat $\hat{X}_i$ means that, that term is missing from the argument (since $\omega$ is a $k$-form, it can only take $k$ vector fields as arguments, so we omit one of them and denote it by hat). In any case, this expression looks extremely ghastly \emoji{skull}\\[0.2cm]
\textbf{Example:}\\[0.2cm]
\begin{itemize}
    \item $\omega \in \Lambda^0\SM = \cty{\SM}$. Then, the second term cannot happen as $\omega$ does not take any argument. We get:
    $$d\omega = 1\times (-1)^{2}X\omega = X\omega$$
    This resembles the differential of a function and hence for a $0$-form, the exterior derivative simply gives the differential of the function $\omega$.
    \item $\omega \in \Lambda^1\SM$. Then we get:
    $$d\omega(X_1, X_2) = \frac{1}{2}\qty[X_1\omega(X_2) - X_2\omega(X_1) -\omega(\comtr{X_1}{X_2})]$$
\item $\omega \in \Lambda^2\SM$. Then we get:
\begin{align*}
    d\omega(X_1, X_2,X_3) &= \frac{1}{3}\Bigg[X_1\omega(X_2,X_3) -X_2\omega(X_1,X_3)+X_3\omega(X_1,X_2)\\&\qquad\quad -\omega(\comtr{X_1}{X_2}, X_3)-\omega(\comtr{X_2}{X_3}, X_1) + \omega(\comtr{X_1}{X_3}, X_2)\Bigg]\\
    &= \frac{1}{3}\Bigg[X_1\omega(X_2,X_3) +X_2\omega(X_3,X_1)+X_3\omega(X_1,X_2)\\&\qquad\quad -\omega(\comtr{X_1}{X_2}, X_3)-\omega(\comtr{X_2}{X_3}, X_1) - \omega(\comtr{X_3}{X_1}, X_2)\Bigg]
\end{align*}
\end{itemize}
\begin{lemma}
   If $\omega\in\Lambda^k\SM$ and $f\in \Lambda^0\SM$, 
   $$d(f\omega) = fd\omega + d\ext{f}{\omega}$$
\end{lemma}
\textit{Proof.} From the definition of the exterior derivative, we will have:
\begin{align*}
    (k+1)d(f\omega) (X_1,\ldots,X_{k+1})&= \sum\limits_{i=1}^{k+1} (-1)^{k+1}X_i (f\omega)(X_1,\ldots \widehat{X}_i\ldots, X_{k+1})\\
    &+\qquad \sum\limits_{i<j} (-1)^{i+j}(f\omega)(\comtr{X_i}{X_j}, X_1,\ldots \widehat{X}_i\ldots \widehat{X}_j\ldots X_{k+1})\\
    &=\sum\limits_{i=1}^{k+1} (-1)^{k+1} (fX_i\omega(X_1,\ldots \widehat{X}_i\ldots, X_{k+1}) + (X_if)\omega(X_1,\ldots \widehat{X}_i\ldots, X_{k+1}))\\
    &\qquad +\sum\limits_{i<j} (-1)^{i+j}(f\omega)(\comtr{X_i}{X_j}, X_1,\ldots \widehat{X}_i\ldots \widehat{X}_j\ldots X_{k+1})\\
    &=(k+1)fd\omega(X_1,\ldots, X_{k+1}) +\sum\limits_{i=1}^{k+1}(-1)^{i+1}(X_if)\omega(X_1,\ldots \widehat{X}_i\ldots, X_{k+1})\\
    &=(k+1)fd\omega(X_1,\ldots, X_{k+1}) +\sum\limits_{i=1}^{k+1}(-1)^{i+1}df(X_i)\omega(X_1,\ldots \widehat{X}_i\ldots, X_{k+1})\\
    &=(k+1)fd\omega(X_1,\ldots, X_{k+1}) +\sum\limits_{i=1}^{k+1}(-1)^{i+1}(df\otimes\omega)(X_i,X_1,\ldots \widehat{X}_i\ldots, X_{k+1})\\
    &=(k+1)(fd\omega + \ext{df}{\omega})(X_1,\ldots, X_{k+1}) 
\end{align*}
We obtained the last line from the second last line using the following:
\begin{itemize}
    \item Note that the LHS is anti-symmetric in all its arguments since exterior derivative is a $k+1$ form. 
    \item The first term on the RHS is also anti-symmetric in its arguments. 
    \item Thus, remaining term is antisymmetric too. Then if we denote the term by $\kappa$, then due to property of being anti-symmetric, $\SA\kappa = \kappa$ but if we do $\SA\kappa$, by linearity of $\SA$, we will get the term $\SA(df\otimes\omega) = df\wedge \omega$
\end{itemize}
Thus, from this, we obtained that kind of the Liebniz rule for the exterior derivative:
$$d(f\omega) = fd\omega + df\wedge \omega$$\\
\textbf{Coordinate Representation:}\\[0.2cm]
Working in a coordinate system greatly simplifies things in this case. For that, consider $\omega = \omega_{i_1\ldots i_k}dx^{i_1}\wedge\ldots\wedge x^{i_k}$ in some coordinate system $(x^1,\ldots,x^n)$.\\[0.2cm]
Then, using the above ``product rule'', we get:
\begin{align*}
    d\omega = d(\omega_{i_1,\ldots,i_{k}})\wedge dx^{i_1}\wedge\ldots\wedge dx^{i_k} + \omega_{i_1,\ldots,i_{k}} d(dx^{i_1}\wedge\ldots\wedge dx^{i_k})
\end{align*}
The second term can be shown to be zero because:
\begin{align*}
    &(k+1)d(dx^{i_1}\wedge \ldots \wedge dx^{i_k}) \qty(\pdv{x^{i_1}},\ldots,\pdv{x^{i_{k+1}}})\\&= \sum\limits_{n=1}^{k+1}(-1)^{n+1}\pdv{x^{j_n}}\qty(dx^{i_1}\wedge \ldots \wedge dx^{i_k}\qty(\pdv{x^{j_1}}, \ldots\widehat{\pdv{x^{j_n}}}\ldots \pdv{x^{j_{k+1}}}))+\\
    &\quad\ \sum\limits_{m<n} \ldots \qty(\comtr{\pdv{x^{j_m}}}{\pdv{x^{j_n}}})\ldots
\end{align*}
The second term becomes zero since Lie Bracket of the coordinate differentials is zero. In the first term, when $dx^{i_n}$ acts on some $\pdv{x^{j_n}}$, it will produce either zero or one, which is constant, so will give 0 with $\pdv{x^{j_m}}$. Hence, the first term also evaluates to zero. Thus, from the above fact, we obtain:
$$d\omega = d\omega_{i_1,\ldots,i_{k}}\wedge dx^{i_1}\wedge\ldots\wedge dx^{i_k}$$
% Now, note that the Lie Bracket of coordinate differentials is always zero, that is, $\comtr{\pdv{x^i}}{\pdv{x^j}}=0$ (proved earlier). Then for the $i<j$ sum, we will get some terms of the form $\omega(0,\ldots)$ which, by the liearity of $\omega$, is always zero. Hence, in the definition of the exterior derivative if we take $X_i = \pdv{x^i}$, only the first term survives. Thus we obtain:
% \begin{align*}
%     (d\omega)_{i_1\ldots i_{k+1}} &=d\omega\qty(\pdv{x^{i_1}},\ldots,\pdv{x^{i_{k+1}}})\\
%     &=\frac{1}{k+1}\sum\limits_{a=1}^{k+1} (-1)^{a+1} \pdv{x^{i_a}}\omega_{i_1,\ldots\hat{i}_a\ldots i_{k+1}}
% \end{align*}
% In the coordinate representation, we have:
% \begin{align*}
%     d\omega &= (d\omega)_{i_1,\ldots,i_{k+1}} dx^{i_1}\wedge\ldots\wedge dx^{i_{k+1}}\\
%    &= \frac{1}{k+1}\sum\limits_{a=1}^{k+1} (-1)^{a+1} \pdv{x^{i_a}}\omega_{i_1,\ldots\hat{i}_a\ldots i_{k+1}} dx^{i_1}\wedge\ldots\wedge dx^{i_{k+1}}\\
%    &=\frac{1}{k+1}\sum\limits_{a=1}^{k+1} \cancel{(-1)^{a+1} }\pdv{x^{i_a}}\omega_{i_1,\ldots\hat{i}_a\ldots i_{k+1}} \ \cancel{(-1)^{a-1}}dx^{i_a}\wedge dx^{i_1}\wedge\ldots \widehat{dx^{i_a}}\ldots\wedge dx^{i_{k+1}}\\
%    &=\frac{1}{k+1}\sum\limits_{a=1}^{k+1} \qty(\pdv{x^{i_a}}\omega_{i_1,\ldots\hat{i}_a\ldots i_{k+1}} dx^{i_a})\wedge dx^{i_1}\wedge\ldots \widehat{dx^{i_a}}\ldots\wedge dx^{i_{k+1}}\\
%    &=\frac{1}{k+1}\sum\limits_{a=1}^{k+1} (d\omega)_{i_1\ldots \ldots\hat{i}_a i_{k}}
% \end{align*}
% \textbf{\textcolor{red}{Proof left, continue later!}}
\begin{lemma}[Graded Liebniz Rule]
    If $\omega \in \Lambda^k\SM$ and $\eta\in \Lambda^l\SM$, we have:
    $$d(\omega \wedge \eta) = d\omega\wedge\eta + (-1)^k\omega\wedge d\eta$$
\end{lemma}
\textit{Proof.} Let us use the coordinate version to express $\eta$ and $\omega$. Then we have:
\begin{align*}
    \omega &= \omega_{i_1\ldots i_k} dx^{i_1}\wedge\ldots\wedge dx^{i_k}\\
     \eta &= \eta_{i_1\ldots i_l} dx^{i_1}\wedge\ldots\wedge dx^{i_l}
\end{align*}
Then using the product rule, we have:
\begin{align*}
    d(\omega\wedge \eta) &= d(\omega_{i_1\ldots i_k}\eta_{i_1\ldots i_l} dx^{i_1}\wedge\ldots\wedge dx^{i_k}\wedge dx^{i_1}\wedge\ldots\wedge dx^{i_l})\\
    &=d(\omega_{i_1\ldots i_k}\eta_{i_1\ldots i_l})\wedge dx^{i_1}\wedge\ldots\wedge dx^{i_k}\wedge dx^{i_1}\wedge\ldots\wedge dx^{i_l}\\
    &=d(\omega_{i_1\ldots i_k})\eta_{i_1\ldots i_l}\wedge dx^{i_1}\wedge\ldots\wedge dx^{i_k}\wedge dx^{i_1}\wedge\ldots\wedge dx^{i_l}+\\
    &\quad \omega_{i_1\ldots i_k}d(\eta_{i_1\ldots i_l})\wedge dx^{i_1}\wedge\ldots\wedge dx^{i_k}\wedge dx^{i_1}\wedge\ldots\wedge dx^{i_l}\\
    &=d(\omega_{i_1\ldots i_k})\wedge dx^{i_1}\wedge\ldots\wedge dx^{i_k}\wedge \eta_{i_1\ldots i_l}\wedge dx^{i_1}\wedge\ldots\wedge dx^{i_l}\\
    &\quad (-1)^k \omega_{i_1\ldots i_k}\wedge dx^{i_1}\wedge\ldots\wedge dx^{i_k} d(\eta_{i_1\ldots i_l})\wedge dx^{i_1}\wedge\ldots\wedge dx^{i_l}\\
    &=d\omega\wedge \eta + (-1)^k \omega\wedge d\eta
\end{align*}
Note that in the second last step, we had to introduct $(-1)^k$ since $d(\eta_{i_1\ldots i_l})$ is a one-form and we had to shift it over $k$ indices. \\[0.2cm]
If $d(\omega\wedge \eta) =0$ then $\omega\wedge \eta$ is called a \textit{closed form}. 
\begin{lemma}
   $$ d^2\omega = 0 \ \ \forall \ \omega \in \Lambda^k\SM$$
\end{lemma}
\textit{Proof.} Given $\omega =\omega_{i_1\ldots i_k}x^{i_1}\wedge \ldots \wedge x^{i_k}$, we have:
\begin{align*}
    d\omega &= d(\omega_{i_1\ldots i_k}) x^{i_1}\wedge \ldots \wedge x^{i_k}\\
    &=\qty(\pdv{\omega_{i_1\ldots i_k}}{x^k})dx^k\wedge x^{i_1}\wedge \ldots \wedge x^{i_k}
\end{align*}
Now, applying the exterior derivative once again, we get:
\begin{align*}
    d^2\omega &= d\qty(\qty(\pdv{\omega_{i_1\ldots i_k}}{x^k})dx^k\wedge x^{i_1}\wedge \ldots \wedge x^{i_k})\\
    &=\qty(\pdv{\omega_{i_1\ldots i_k}}{x^l}{x^k})dx^l\wedge dx^k\wedge x^{i_1}\wedge \ldots \wedge x^{i_k}\\
    &=\sum\limits_{k=l}\qty(\pdv{\omega_{i_1\ldots i_k}}{x^k}{x^k})\cancelto{0}{dx^k\wedge dx^k\wedge} \ldots \\
    &\qquad +\sum\limits_{k<l} \qty(\pdv{\omega_{i_1\ldots i_k}}{x^l}{x^k})dx^l\wedge dx^k \ldots + \sum\limits_{k>l} \qty(\pdv{\omega_{i_1\ldots i_k}}{x^l}{x^k})dx^l\wedge dx^k\ldots \\
    &=\sum\limits_{k<l} \qty(\pdv{\omega_{i_1\ldots i_k}}{x^l}{x^k})dx^l\wedge dx^k \ldots - \sum\limits_{k>l} \qty(\pdv{\omega_{i_1\ldots i_k}}{x^l}{x^k})dx^k\wedge dx^l\ldots\\
    &=\sum\limits_{k<l} \qty(\pdv{\omega_{i_1\ldots i_k}}{x^l}{x^k} - \pdv{\omega_{i_1\ldots i_k}}{x^k}{x^l})dx^l\wedge dx^k \ldots
\end{align*}
Thus, we see the $d\omega = 0\ \forall \ \omega\  \implies d^2 \equiv 0$\\[0.2cm]
\textbf{Some potential use cases...}\\[0.2cm]
We can check (using some boring algebra) that if we take $\re^3$ and calculate the exterior derivative of a one-form, we will obtain the components of the curl. Thus, we can say that the exterior derivative of a one-form generalises the notion of a curl. Also, if we take the exterior derivative of a two-form, we will obtain the components of the gradient. \\[0.2cm]
\textbf{Interesting example: Electromagnetic Tensor}\\[0.2cm]
Modern formalism of electromagnetism treats electric field as a one-form and magnetic field as a two form. Hence, we can write:
\begin{align*}
    E&:= E_x dx + E_y dy + E_z dz\\
B&:= B_x dy\wedge dz + B_y dz\wedge dx + Bz dx\wedge dy
\end{align*}
Then we can define the electromagnetic tensor as the following two-form:
$$F:= B + E\wedge dt$$
Then we will have:
\begin{align*}
    F &= (B_x dy\wedge dz + B_y dz\wedge dx + Bz dx\wedge dy) + (E_x dx + E_y dy + E_z dz)\wedge dt\\
    &=(B_x dy\wedge dz + B_y dz\wedge dx + Bz dx\wedge dy) + E_x dx\wedge dt +E_y dy\wedge dt+E_z dz\wedge dt\\
    &=B_x dy\wedge dz + B_y dz\wedge dx+Bz dx\wedge dy - E_x dt\wedge dx -E_y dt\wedge dy -E_z dt\wedge dz
\end{align*}
From this expression and writing $F = F_{\mu\nu}dx^\mu\wedge dx^\nu$, we can easily obtain the electromagnetic tensor components:
\[
[F]_{\mu\nu} =
\begin{pmatrix}
0 & -E_x & -E_y & -E_z \\
E_x & 0 & B_z & -B_y \\
E_y & -B_z & 0 & B_x \\
E_z & B_y & -B_x & 0
\end{pmatrix}
\]